Java/src/Java/Logic/SpecLogic.v
@@ -9,7 +9,9 @@ Local Existing Instance ILPre_Ops.
 Local Existing Instance ILPre_ILogic.
 *)
 
-Definition spec := ILPreFrm Prog_sub (ILPreFrm ge Prop).
+Require Import AssertionLogic.
+
+Definition spec := ILPreFrm Prog_sub (ILPreFrm ge (ILPreFrm extSP Prop)).
 
 (*
 Global Instance ILLOperatorsSpec : ILLOperators spec := _.
@@ -19,24 +21,26 @@ Global Instance ILSpec : ILLater spec := _.
 
 Local Transparent ILPre_Ops.
 Require Import Compare_dec.
-Definition mk_spec (f: Program -> nat -> Prop)
-  (Hnat: forall k P, f P (S k) -> f P k)
-  (HSPred: forall k P P', Prog_sub P P' -> f P k -> f P' k) : spec.
-  refine (mkILPreFrm (fun k => mkILPreFrm (f k) _) _).
+Definition mk_spec (f: Program -> nat -> sasn -> Prop)
+  (Hnat: forall k P T, f P (S k) T -> f P k T)
+  (HSPred: forall k P P' T, Prog_sub P P' -> f P k T -> f P' k T)
+  (HSExt: forall k P T U, extSP T U -> f P k T -> f P k U) : spec.
+  refine (mkILPreFrm (fun k => (mkILPreFrm (fun P => (mkILPreFrm (fun T => f k P T)) _)) _) _).
 Proof.
-  assert (forall k P P', Prog_sub P P' -> f P k -> f P' k) as HProg.
-  intros k P P' HPP' S'. eapply HSPred; eassumption. 
-  intros p p' Hp'' n S'; simpl in *. eapply HProg; eassumption.
+  intros P P' HPP' k. simpl. intros. eapply HSPred. eassumption. assumption.
   Grab Existential Variables.
-  intros n m Hnk S'. generalize dependent m. induction n; intros.
-  + assert (m = 0) by omega; subst. apply S'.
-  + destruct (gt_eq_gt_dec m (S n)) as [[H | H] | H]; [| | omega].
-    * apply IHn. apply Hnat. apply S'. omega.
-    * subst. apply S'.
+  intros n m Hnk S'. simpl.
+   generalize dependent m. induction n; intros.
+  + assert (m = 0) by omega; subst. apply H.
+  + destruct (gt_eq_gt_dec m (S n)) as [[H1 | H1] | H1]; [| | omega].
+    * apply IHn. omega. apply Hnat. apply H.
+    * subst. apply H.
+  + intros; simpl. apply HSExt; assumption.
+
 Defined.
 
 Program Definition prog_spec (X : Program -> Prop) : spec :=
-  mk_spec (fun (P : Program) _ => forall (Q : Program) , Prog_sub P Q -> X Q /\ valid_program Q = true) _ _.
+  mk_spec (fun (P : Program) _ _ => forall (Q : Program) , Prog_sub P Q -> X Q /\ valid_program Q = true) _ _ _.
 Next Obligation.
   intros; apply H0; etransitivity; eassumption.
 Qed.
@@ -55,7 +59,7 @@ Definition prog_eq Prog : spec := [prog] (fun P => P = Prog).
 
 Lemma prog_eq_to_prop P (f : Program -> Prop) (H : f P) : prog_eq P |-- [prog] f.
 Proof.
-  intros Q n HQ R HQR.
+  intros Q n T HQ R HQR.
   specialize (HQ _ HQR).
   simpl in *. subst. intuition congruence.
 Qed.
